feat: preserve outer sum eight witness

ReverseAddBoundary.fst
@@ -520,6 +520,34 @@ let local_profile_witness_450822227944 () : Lemma (
   no_overflow_outer_sum_1_to_4_cell_implies_next_witness source;
   ()
 
+let trace_profile_450822227944 () : Lemma (
+    trace_digits [4; 4; 9; 7; 2; 2; 2; 2; 8; 0; 5; 4] ==
+      [8; 9; 9; 5; 5; 4; 4; 4; 5; 0; 0; 9] /\
+    trace_carries [4; 4; 9; 7; 2; 2; 2; 2; 8; 0; 5; 4] ==
+      [0; 0; 0; 0; 1; 0; 0; 0; 0; 1; 1; 1; 0] /\
+    length (trace_digits [4; 4; 9; 7; 2; 2; 2; 2; 8; 0; 5; 4]) ==
+      length [4; 4; 9; 7; 2; 2; 2; 2; 8; 0; 5; 4] /\
+    nth (trace_carries [4; 4; 9; 7; 2; 2; 2; 2; 8; 0; 5; 4])
+      (length [4; 4; 9; 7; 2; 2; 2; 2; 8; 0; 5; 4]) == Some 0 /\
+    trace_sum_at [4; 4; 9; 7; 2; 2; 2; 2; 8; 0; 5; 4] 0 == 8) =
+  assert (trace_digits [4; 4; 9; 7; 2; 2; 2; 2; 8; 0; 5; 4] ==
+    [8; 9; 9; 5; 5; 4; 4; 4; 5; 0; 0; 9]);
+  assert (trace_carries [4; 4; 9; 7; 2; 2; 2; 2; 8; 0; 5; 4] ==
+    [0; 0; 0; 0; 1; 0; 0; 0; 0; 1; 1; 1; 0]);
+  assert (trace_sum_at [4; 4; 9; 7; 2; 2; 2; 2; 8; 0; 5; 4] 0 == 8);
+  ()
+
+let local_profile_witness_900544455998 () : Lemma (
+    trace_local_profile_complement_witness
+      [8; 9; 9; 5; 5; 4; 4; 4; 5; 0; 0; 9]) =
+  assert (canonical #10 [4; 4; 9; 7; 2; 2; 2; 2; 8; 0; 5; 4]);
+  assert ([4; 4; 9; 7; 2; 2; 2; 2; 8; 0; 5; 4] <> []);
+  trace_profile_450822227944 ();
+  reverse_add_450822227944_to_900544455998 ();
+  no_overflow_outer_sum_6_to_9_implies_next_witness
+    [4; 4; 9; 7; 2; 2; 2; 2; 8; 0; 5; 4];
+  ()
+
 let trace_palindrome_obstruction_60744805 () : Lemma (
     trace_palindrome_obstruction [5; 0; 8; 4; 4; 7; 0; 6]) =
   trace_palindrome_obstruction_at_60744805 ();
